aarch64: updates for GICv3 split EOI mode
Brings changes for split EOI (End Of Interrupt) mode from seL4/seL4#1183
into the verification.

Most of what changes in the seL4 pull request is underneath the machine
interface and implements a different mechanism for masking/unmasking
interrupts (using priority drop instead of actual masking/unmasking).
For the purposes of the proof, what we want from the hardware remains
the same: when deactivated, the interrupt will no longer fire.

Signed-off-by: Gerwin Klein <gerwin.klein@proofcraft.systems>

spec/haskell/src/SEL4/Machine/Hardware.lhs
@@ -66,7 +66,7 @@ Depending on the architecture, real physical addresses may be the same as the ad
 
 An interrupt request from an external device, or from the CPU's timer, is represented by the type "IRQ".
 
-> newtype IRQ = IRQ Arch.IRQ
+> newtype IRQ = IRQ { theIRQ :: Arch.IRQ }
 >     deriving (Enum, Bounded, Ord, Ix, Eq, Show)
 
 The maximum and minimum IRQ are given explicit constant names here. In Haskell, these are extracted from instantiation of IRQ into the Bounded class. In the formalisation, these constants are generated and defined in Kernel_Config.thy.
